replace hacl64-bignum with generic bignum

code/curve25519/Hacl.Impl.Curve25519.Field64.Hacl.fst
@@ -10,81 +10,71 @@ open Lib.Buffer
 
 module B = Lib.Buffer
 module ST = FStar.HyperStack.ST
+module BSeq = Lib.ByteSequence
+module LSeq = Lib.Sequence
 
-open Hacl.Spec.Curve25519.Field64.Core
+module CD = Hacl.Spec.Curve25519.Field64.Definition
+module CC = Hacl.Spec.Curve25519.Field64.Core
 
-#set-options "--z3rlimit 20 --max_fuel 0 --max_ifuel 0"
+module BN = Hacl.Bignum
+module BD = Hacl.Bignum.Definitions
+module SB = Hacl.Spec.Bignum
+module SD = Hacl.Spec.Bignum.Definitions
+
+#set-options "--z3rlimit 50 --fuel 0 --ifuel 0"
+
 
 [@CInline]
 let add1_ out f1 f2 =
-  let f10 = f1.(0ul) in
-  let f11 = f1.(1ul) in
-  let f12 = f1.(2ul) in
-  let f13 = f1.(3ul) in
-  let carry, (o0, o1, o2, o3) =
-    add1 (f10, f11, f12, f13) f2 in
-  out.(0ul) <- o0;
-  out.(1ul) <- o1;
-  out.(2ul) <- o2;
-  out.(3ul) <- o3;
-  carry
+  let h0 = ST.get () in
+  let c = BN.bn_add1 4ul f1 f2 out in
+  let h1 = ST.get () in
+  assert (let c1, r1 = CC.add1 (as_seq h0 f1) f2 in c == c1 /\ as_seq h1 out == r1);
+  CD.bn_v_is_as_nat (as_seq h0 f1);
+  CD.bn_v_is_as_nat (as_seq h1 out);
+  c
+
 
 [@CInline]
 let fadd_ out f1 f2 =
-  let f10 = f1.(0ul) in
-  let f11 = f1.(1ul) in
-  let f12 = f1.(2ul) in
-  let f13 = f1.(3ul) in
+  let h0 = ST.get () in
+  let c0 = BN.bn_add_eq_len 4ul f1 f2 out in
+  let c = BN.bn_add1 4ul out (c0 *. u64 38) out in
+  out.(0ul) <- out.(0ul) +. c *. u64 38;
+  let h1 = ST.get () in
+  assert (as_seq h1 out == CC.fadd4 (as_seq h0 f1) (as_seq h0 f2));
+  CD.bn_v_is_as_nat (as_seq h0 f1);
+  CD.bn_v_is_as_nat (as_seq h0 f2);
+  CD.bn_v_is_as_nat (as_seq h1 out)
 
-  let f20 = f2.(0ul) in
-  let f21 = f2.(1ul) in
-  let f22 = f2.(2ul) in
-  let f23 = f2.(3ul) in
-
-  let (o0, o1, o2, o3) =
-    fadd4 (f10, f11, f12, f13) (f20, f21, f22, f23) in
-  out.(0ul) <- o0;
-  out.(1ul) <- o1;
-  out.(2ul) <- o2;
-  out.(3ul) <- o3
 
 [@CInline]
 let fsub_ out f1 f2 =
-  let f10 = f1.(0ul) in
-  let f11 = f1.(1ul) in
-  let f12 = f1.(2ul) in
-  let f13 = f1.(3ul) in
+  let h0 = ST.get () in
+  let c0 = BN.bn_sub_eq_len 4ul f1 f2 out in
+  let c = BN.bn_sub1 4ul out (c0 *! u64 38) out in
+  out.(0ul) <- out.(0ul) -. c *. u64 38;
+  let h1 = ST.get () in
+  assert (as_seq h1 out == CC.fsub4 (as_seq h0 f1) (as_seq h0 f2));
+  CD.bn_v_is_as_nat (as_seq h0 f1);
+  CD.bn_v_is_as_nat (as_seq h0 f2);
+  CD.bn_v_is_as_nat (as_seq h1 out)
 
-  let f20 = f2.(0ul) in
-  let f21 = f2.(1ul) in
-  let f22 = f2.(2ul) in
-  let f23 = f2.(3ul) in
-
-  let (o0, o1, o2, o3) =
-    fsub4 (f10, f11, f12, f13) (f20, f21, f22, f23) in
-  out.(0ul) <- o0;
-  out.(1ul) <- o1;
-  out.(2ul) <- o2;
-  out.(3ul) <- o3
 
 [@CInline]
 let fmul_ out f1 f2 tmp =
-  let f10 = f1.(0ul) in
-  let f11 = f1.(1ul) in
-  let f12 = f1.(2ul) in
-  let f13 = f1.(3ul) in
+  let h0 = ST.get () in
+  let tmp0 = sub tmp 0ul 8ul in
+  BN.bn_mul 4ul 4ul f1 f2 tmp0;
+  let c0 = BN.bn_mul1_lshift_add_in_place 4ul (sub tmp0 4ul 4ul) (u64 38) 4ul 0ul (sub tmp0 0ul 4ul) in
+  let c = BN.bn_add1 4ul (sub tmp0 0ul 4ul) (c0 *. u64 38) out in
+  out.(0ul) <- out.(0ul) +. c *. u64 38;
+  let h1 = ST.get () in
+  assert (as_seq h1 out == CC.fmul4 (as_seq h0 f1) (as_seq h0 f2));
+  CD.bn_v_is_as_nat (as_seq h0 f1);
+  CD.bn_v_is_as_nat (as_seq h0 f2);
+  CD.bn_v_is_as_nat (as_seq h1 out)
 
-  let f20 = f2.(0ul) in
-  let f21 = f2.(1ul) in
-  let f22 = f2.(2ul) in
-  let f23 = f2.(3ul) in
-
-  let (o0, o1, o2, o3) =
-    fmul4 (f10, f11, f12, f13) (f20, f21, f22, f23) in
-  out.(0ul) <- o0;
-  out.(1ul) <- o1;
-  out.(2ul) <- o2;
-  out.(3ul) <- o3
 
 [@CInline]
 let fmul2_ out f1 f2 tmp =
@@ -97,53 +87,42 @@ let fmul2_ out f1 f2 tmp =
   fmul_ out1 f11 f21 tmp;
   fmul_ out2 f12 f22 tmp
 
+
 [@CInline]
 let fmul1_ out f1 f2 =
-  let f10 = f1.(0ul) in
-  let f11 = f1.(1ul) in
-  let f12 = f1.(2ul) in
-  let f13 = f1.(3ul) in
+  let h0 = ST.get () in
+  let c0 = BN.bn_mul1 4ul f1 f2 out in
+  let c = BN.bn_add1 4ul out (c0 *. u64 38) out in
+  out.(0ul) <- out.(0ul) +. c *. u64 38;
+  let h1 = ST.get () in
+  assert (as_seq h1 out == CC.fmul14 (as_seq h0 f1) f2);
+  CD.bn_v_is_as_nat (as_seq h0 f1);
+  CD.bn_v_is_as_nat (as_seq h1 out)
 
-  let (o0, o1, o2, o3) = fmul14 (f10, f11, f12, f13) f2 in
-  out.(0ul) <- o0;
-  out.(1ul) <- o1;
-  out.(2ul) <- o2;
-  out.(3ul) <- o3
 
 [@CInline]
 let fsqr_ out f1 tmp =
-  push_frame ();
-  let tmp = create 16ul (u64 0) in
-  fmul_ out f1 f1 tmp;
-  pop_frame ()
+  let h0 = ST.get () in
+  BN.bn_sqr 4ul f1 tmp;
+  SB.bn_sqr_lemma (as_seq h0 f1);
+  let c0 = BN.bn_mul1_lshift_add_in_place 4ul (sub tmp 4ul 4ul) (u64 38) 4ul 0ul (sub tmp 0ul 4ul) in
+  let c = BN.bn_add1 4ul (sub tmp 0ul 4ul) (c0 *. u64 38) out in
+  out.(0ul) <- out.(0ul) +. c *. u64 38;
+  let h1 = ST.get () in
+  assert (as_seq h1 out == CC.fsqr4 (as_seq h0 f1));
+  CD.bn_v_is_as_nat (as_seq h0 f1);
+  CD.bn_v_is_as_nat (as_seq h1 out)
+
 
 [@CInline]
 let fsqr2_ out f tmp =
-  fmul2_ out f f tmp
+  let out1 = B.sub out 0ul 4ul in
+  let out2 = B.sub out 4ul 4ul in
+  let f1 = B.sub f 0ul 4ul in
+  let f2 = B.sub f 4ul 4ul in
+  fmul_ out1 f1 f1 tmp;
+  fmul_ out2 f2 f2 tmp
 
-val lemma_cswap2_step:
-    bit:uint64{v bit <= 1}
-  -> p1:uint64
-  -> p2:uint64
-  -> Lemma (
-      let mask = u64 0 -. bit in
-      let dummy = mask &. (p1 ^. p2) in
-      let p1' = p1 ^. dummy in
-      let p2' = p2 ^. dummy in
-      if v bit = 1 then p1' == p2 /\ p2' == p1 else p1' == p1 /\ p2' == p2)
-let lemma_cswap2_step bit p1 p2 =
-  let mask = u64 0 -. bit in
-  assert (v bit == 0 ==> v mask == 0);
-  assert (v bit == 1 ==> v mask == pow2 64 - 1);
-  let dummy = mask &. (p1 ^. p2) in
-  logand_lemma mask (p1 ^. p2);
-  assert (v bit == 1 ==> v dummy == v (p1 ^. p2));
-  assert (v bit == 0 ==> v dummy == 0);
-  let p1' = p1 ^. dummy in
-  assert (v dummy == v (if v bit = 1 then (p1 ^. p2) else u64 0));
-  logxor_lemma p1 p2;
-  let p2' = p2 ^. dummy in
-  logxor_lemma p2 p1
 
 [@CInline]
 let cswap2_ bit p1 p2 =
@@ -165,8 +144,10 @@ let cswap2_ bit p1 p2 =
       let dummy = mask &. (p1.(i) ^. p2.(i)) in
       p1.(i) <- p1.(i) ^. dummy;
       p2.(i) <- p2.(i) ^. dummy;
-      lemma_cswap2_step bit ((as_seq h0 p1).[v i]) ((as_seq h0 p2).[v i])
+      Hacl.Spec.Bignum.Lib.lemma_cswap2_step bit ((as_seq h0 p1).[v i]) ((as_seq h0 p2).[v i])
     );
   let h1 = ST.get () in
-  Lib.Sequence.eq_intro (as_seq h1 p1) (if v bit = 1 then as_seq h0 p2 else as_seq h0 p1);
-  Lib.Sequence.eq_intro (as_seq h1 p2) (if v bit = 1 then as_seq h0 p1 else as_seq h0 p2)
+  assert (if v bit = 1 then (eq_intro (as_seq h1 p1) (as_seq h0 p2); as_seq h1 p1 == as_seq h0 p2)
+    else (eq_intro (as_seq h1 p1) (as_seq h0 p1); as_seq h1 p1 == as_seq h0 p1));
+  assert (if v bit = 1 then (eq_intro (as_seq h1 p2) (as_seq h0 p1); as_seq h1 p2 == as_seq h0 p1)
+    else (eq_intro (as_seq h1 p2) (as_seq h0 p2); as_seq h1 p2 == as_seq h0 p2))
