code/curve25519/Hacl.Impl.Curve25519.Field64.fst
@@ -17,13 +17,15 @@ module BSeq = Lib.ByteSequence
 module P = Spec.Curve25519
 module S = Hacl.Spec.Curve25519.Field64.Definition
 module SC = Hacl.Spec.Curve25519.Field64
+module SD = Hacl.Spec.Bignum.Definitions
 
-let u256 = lbuffer uint64 4ul
-let u512 = lbuffer uint64 8ul
-let u1024 = lbuffer uint64 16ul
+#reset-options "--z3rlimit 50 --fuel 0 --ifuel 0"
+
+let felem = lbuffer uint64 4ul
+let felem2 = lbuffer uint64 8ul
 
 noextract
-let as_nat (h:mem) (e:u256) : GTot nat =
+let as_nat (h:mem) (e:felem) : GTot nat =
   let s = as_seq h e in
   let s0 = s.[0] in
   let s1 = s.[1] in
@@ -32,58 +34,31 @@ let as_nat (h:mem) (e:u256) : GTot nat =
   S.as_nat4 (s0, s1, s2, s3)
 
 noextract
-let wide_as_nat (h:mem) (e:u512) : GTot nat =
-  let s = as_seq h e in
-  let s0 = s.[0] in
-  let s1 = s.[1] in
-  let s2 = s.[2] in
-  let s3 = s.[3] in
-  let s4 = s.[4] in
-  let s5 = s.[5] in
-  let s6 = s.[6] in
-  let s7 = s.[7] in
-  S.wide_as_nat4 (s0, s1, s2, s3, s4, s5, s6, s7)
+let fevalh (h:mem) (f:felem) : GTot P.elem = (as_nat h f) % P.prime
 
-noextract
-let fevalh (h:mem) (f:u256) : GTot P.elem = (as_nat h f) % P.prime
-
-noextract
-let feval_wideh (h:mem) (f:u512) : GTot P.elem = (wide_as_nat h f) % P.prime
-
-#reset-options "--z3rlimit 50 --record_options"
-
-let felem = lbuffer uint64 4ul
-let felem2 = lbuffer uint64 8ul
-let felem_wide = lbuffer uint64 8ul
-
-noextract
-let as_tup4 (h:mem) (f:felem) : GTot S.felem4 =
-  let s = as_seq h f in
-  let s0 = s.[0] in
-  let s1 = s.[1] in
-  let s2 = s.[2] in
-  let s3 = s.[3] in
-  (s0, s1, s2, s3)
 
 inline_for_extraction noextract
-val create_felem:
-  unit -> StackInline felem
+val create_felem: unit ->
+  StackInline felem
   (requires fun _ -> True)
   (ensures  fun h0 f h1 ->
     stack_allocated f h0 h1 (Seq.create 4 (u64 0)) /\
     as_nat h1 f == 0)
+
 let create_felem () = create 4ul (u64 0)
+
 
 inline_for_extraction noextract
 val load_felem:
     f:felem
-  -> u64s:lbuffer uint64 4ul
-  -> Stack unit
-    (requires fun h ->
-      live h u64s /\ live h f /\ disjoint u64s f)
-    (ensures  fun h0 _ h1 ->
-      modifies (loc f) h0 h1 /\
-      as_nat h1 f == BSeq.nat_from_intseq_le (as_seq h0 u64s))
+  -> u64s:lbuffer uint64 4ul ->
+  Stack unit
+  (requires fun h ->
+    live h u64s /\ live h f /\ disjoint u64s f)
+  (ensures  fun h0 _ h1 ->
+    modifies (loc f) h0 h1 /\
+    as_nat h1 f == BSeq.nat_from_intseq_le (as_seq h0 u64s))
+
 let load_felem f u64s =
   let h0 = ST.get () in
   Hacl.Impl.Curve25519.Lemmas.lemma_nat_from_uints64_le_4 (as_seq h0 u64s);
@@ -92,45 +67,57 @@ let load_felem f u64s =
   f.(2ul) <- u64s.(2ul);
   f.(3ul) <- u64s.(3ul)
 
-val carry_pass_store:
-    f:felem
- -> Stack unit
-   (requires fun h ->
-     live h f)
-   (ensures fun h0 _ h1 ->
-     modifies (loc f) h0 h1 /\
-     as_nat h1 f == S.as_nat4 (SC.carry_pass_store (as_tup4 h0 f)))
+
+val carry_pass_store: f:felem ->
+  Stack unit
+  (requires fun h -> live h f)
+  (ensures fun h0 _ h1 ->
+    modifies (loc f) h0 h1 /\
+    as_seq h1 f == SC.carry_pass_store (as_seq h0 f))
+
 [@ Meta.Attribute.inline_ ]
 let carry_pass_store f =
   let f3 = f.(3ul) in
   let top_bit = f3 >>. 63ul in
   f.(3ul) <- f3 &. u64 0x7fffffffffffffff;
-  let carry = add1 f f (u64 19 *! top_bit) in ()
+  let h0 = ST.get () in
+  let carry = add1 f f (u64 19 *! top_bit) in
+  let h1 = ST.get () in
+  assert (as_nat h1 f + v carry * pow2 256 == as_nat h0 f + 19 * v top_bit);
+  S.bn_v_is_as_nat (as_seq h1 f);
+  S.bn_v_is_as_nat (as_seq h0 f);
+  let cr = Ghost.hide (Hacl.Spec.Curve25519.Field64.Core.add1 (as_seq h0 f) (u64 19 *! top_bit)) in
+  SD.bn_eval_bound (snd cr) 4;
+  assert (v (fst cr) == v carry /\ SD.bn_v (snd cr) == as_nat h1 f);
+  SD.bn_eval_inj 4 (snd cr) (as_seq h1 f);
+  ()
+
 
 val store_felem:
     u64s:lbuffer uint64 4ul
-  -> f:felem
-  -> Stack unit
-    (requires fun h ->
-      live h f /\ live h u64s /\ disjoint u64s f)
-    (ensures  fun h0 _ h1 ->
-      modifies (loc u64s |+| loc f) h0 h1 /\
-      as_seq h1 u64s == BSeq.nat_to_intseq_le 4 (fevalh h0 f))
+  -> f:felem ->
+  Stack unit
+  (requires fun h ->
+    live h f /\ live h u64s /\ disjoint u64s f)
+  (ensures  fun h0 _ h1 ->
+    modifies (loc u64s |+| loc f) h0 h1 /\
+    as_seq h1 u64s == BSeq.nat_to_intseq_le 4 (fevalh h0 f))
+
 [@ Meta.Attribute.inline_ ]
 let store_felem u64s f =
   let h0 = ST.get () in
   carry_pass_store f;
   let h1 = ST.get () in
-  SC.lemma_carry_pass_store0 (as_tup4 h0 f);
+  SC.lemma_carry_pass_store_first (as_seq h0 f);
   carry_pass_store f;
   let h2 = ST.get () in
-  SC.lemma_carry_pass_store1 (as_tup4 h1 f);
+  SC.lemma_carry_pass_store_second (as_seq h1 f);
   let f0 = f.(0ul) in
   let f1 = f.(1ul) in
   let f2 = f.(2ul) in
   let f3 = f.(3ul) in
-  assert (v f3 < pow2 63);
-  assert (as_nat h2 f < pow2 255);
+  S.bn_v_is_as_nat (as_seq h0 f);
+  S.bn_v_is_as_nat (as_seq h2 f);
   let (o0, o1, o2, o3) = SC.subtract_p4 (f0, f1, f2, f3) in
   assert (S.as_nat4 (o0, o1, o2, o3) < P.prime);
   assert (S.as_nat4 (o0, o1, o2, o3) == (as_nat h2 f) % P.prime);
@@ -142,42 +129,48 @@ let store_felem u64s f =
   Hacl.Impl.Curve25519.Lemmas.lemma_nat_from_uints64_le_4 (as_seq h3 u64s);
   BSeq.lemma_nat_from_to_intseq_le_preserves_value 4 (as_seq h3 u64s)
 
+
 inline_for_extraction noextract
-val set_zero:
-  f:felem -> Stack unit
+val set_zero: f:felem ->
+  Stack unit
   (requires fun h -> live h f)
   (ensures  fun h0 _ h1 ->
     modifies (loc f) h0 h1 /\
     as_nat h1 f == 0)
+
 let set_zero f =
   f.(0ul) <- u64 0;
   f.(1ul) <- u64 0;
   f.(2ul) <- u64 0;
   f.(3ul) <- u64 0
 
+
 inline_for_extraction noextract
-val set_one:
-  f:felem -> Stack unit
+val set_one: f:felem ->
+  Stack unit
   (requires fun h -> live h f)
   (ensures  fun h0 _ h1 ->
     modifies (loc f) h0 h1 /\
     as_nat h1 f == 1)
+
 let set_one f =
   f.(0ul) <- u64 1;
   f.(1ul) <- u64 0;
   f.(2ul) <- u64 0;
   f.(3ul) <- u64 0
 
+
 inline_for_extraction noextract
 val copy_felem:
     f1:felem
-  -> f2:felem
-  -> Stack unit
-    (requires fun h ->
-      live h f1 /\ live h f2 /\ disjoint f1 f2)
-    (ensures  fun h0 _ h1 ->
-      modifies (loc f1) h0 h1 /\
-      as_seq h1 f1 == as_seq h0 f2)
+  -> f2:felem ->
+  Stack unit
+  (requires fun h ->
+    live h f1 /\ live h f2 /\ disjoint f1 f2)
+  (ensures  fun h0 _ h1 ->
+    modifies (loc f1) h0 h1 /\
+    as_seq h1 f1 == as_seq h0 f2)
+
 let copy_felem f1 f2 =
   f1.(0ul) <- f2.(0ul);
   f1.(1ul) <- f2.(1ul);
